msl/ghost_seplog.v
@@ -8,14 +8,13 @@ Local Open Scope logic.
 
 Class BupdSepLog (A N D: Type) {ND: NatDed A}{SL: SepLog A} := mkBSL {
   bupd: A -> A;
-  inG: Ghost -> A;
   own: forall {RA: Ghost}, N -> G -> D -> A;
   bupd_intro: forall P, P |-- bupd P;
   bupd_mono: forall P Q, P |-- Q -> bupd P |-- bupd Q;
   bupd_trans: forall P, bupd (bupd P) |-- bupd P;
   bupd_frame_r: forall P Q, bupd P * Q |-- bupd (P * Q);
   own_alloc: forall {RA: Ghost} a pp, valid a ->
-    inG RA |-- bupd (EX g: N, own g a pp);
+    emp |-- bupd (EX g: N, own g a pp);
   own_op: forall {RA: Ghost} g (a1 a2 a3: G) pp, join a1 a2 a3 ->
     own g a3 pp = own g a1 pp * own g a2 pp;
   own_valid_2: forall {RA: Ghost} g (a1 a2: G) pp,
@@ -23,9 +22,7 @@ Class BupdSepLog (A N D: Type) {ND: NatDed A}{SL: SepLog A} := mkBSL {
   own_update_ND: forall {RA: Ghost} g (a: G) B pp, fp_update_ND a B ->
     own g a pp |-- bupd (EX b : _, !!(B b) && own g b pp);
   own_update: forall {RA: Ghost} g (a: G) b pp, fp_update a b ->
-    own g a pp |-- bupd (own g b pp);
-  inG_emp: forall RA, inG RA |-- emp;
-  inG_dup: forall RA, inG RA |-- inG RA * inG RA
+    own g a pp |-- bupd (own g b pp)
   }.
 
 Notation "|==> P" := (bupd P) (at level 62): logic.
@@ -55,8 +52,8 @@ Qed.
 
 Instance LiftBupdSepLog (A B N D: Type) {NB: NatDed B}{SB: SepLog B}{BSLB: BupdSepLog B N D} :
   BupdSepLog (A -> B) N D.
- apply (mkBSL _ _ _ _ _ (fun P rho => |==> P rho) (fun RA rho => inG RA)
-   (fun RA g a pp rho => own g a pp)); repeat intro; simpl.
+ apply (mkBSL _ _ _ _ _ (fun P rho => |==> P rho) (fun RA g a pp rho => own g a pp));
+   repeat intro; simpl.
  apply bupd_intro.
  apply bupd_mono; auto.
  apply bupd_trans.
@@ -66,6 +63,4 @@ Instance LiftBupdSepLog (A B N D: Type) {NB: NatDed B}{SB: SepLog B}{BSLB: BupdS
  apply own_valid_2.
  apply own_update_ND; auto.
  apply own_update; auto.
- apply inG_emp.
- apply inG_dup.
 Defined.
